Finish DiskLog up to extend

src/PermDiskLog.v
@@ -13,10 +13,11 @@ Require Import FSLayout.
 Require Import Rounding.
 Require Import List ListUtils.
 Require Import Psatz.
-Require Import PermAsyncRecArray.
-Require Export PermDiskLogHdr.
+Require Export PermDiskLogHdr PermAsyncRecArray.
 
 Set Implicit Arguments.
+
+Import ListNotations.
 
 Module DescSig <: RASig.
 
@@ -121,6 +122,13 @@ Fixpoint combine_nonzero (al : list addr) (vl : list tagged_block) : contents :=
   match al, vl with
   | 0 :: al', v :: vl' => combine_nonzero al' vl
   | a :: al', v :: vl' => (a, v) :: (combine_nonzero al' vl')
+  | _, _ => nil
+  end.
+
+Fixpoint combine_nonzero_gen (al : list addr) (vl : list handle) :=
+  match al, vl with
+  | 0 :: al', v :: vl' => combine_nonzero_gen al' vl
+  | a :: al', v :: vl' => (a, v) :: (combine_nonzero_gen al' vl')
   | _, _ => nil
   end.
 
@@ -327,15 +335,16 @@ Definition avail xp cs :=
     let '(_, (ndesc, _), _) := nr in
     Ret ^(cs, ((LogLen xp) - ndesc * DescSig.items_per_val)).
 
+     
   Definition read xp cs :=
     let^ (cs, nr) <- PermDiskLogHdr.read xp cs;;
     let '(_, (ndesc, ndata), _) := nr in
     let^ (cs, ahl) <- Desc.read_all xp ndesc cs;;
     abl <- unseal_all ahl;;
-                   
+    let wal := fold_left DescDefs.iunpack abl nil in               
     let al := map (@wordToNat addrlen) wal in
     let^ (cs, vl) <- Data.read_all xp ndata cs;;
-    Ret ^(cs, combine_nonzero al vl).
+    Ret ^(cs, (al, vl)).
 
   (* this is an evil hint *)
   Remove Hints Forall_nil.
@@ -348,12 +357,12 @@ Definition avail xp cs :=
   Hint Resolve Forall_True.
 
   Lemma combine_nonzero_ok : forall l,
-    combine_nonzero (map fst l) (vals_nonzero l) = log_nonzero l.
+    combine_nonzero (map fst l) (blocks_nonzero l) = log_nonzero l.
   Proof.
-    unfold vals_nonzero.
+    unfold blocks_nonzero.
     induction l; intros; simpl; auto.
     destruct a, n; simpl.
-    case_eq (map ent_valu (log_nonzero l)); intros; simpl.
+    case_eq (map ent_block (log_nonzero l)); intros; simpl.
     apply map_eq_nil in H; auto.
     rewrite <- H; auto.
     rewrite IHl; auto.
@@ -468,7 +477,7 @@ Definition avail xp cs :=
 
   Lemma combine_nonzero_padded_wordToNat : forall l,
     Forall addr_valid l ->
-    combine_nonzero (map (@wordToNat _) (map ent_addr (padded_log l))) (vals_nonzero l) = log_nonzero l.
+    combine_nonzero (map (@wordToNat _) (map ent_addr (padded_log l))) (blocks_nonzero l) = log_nonzero l.
   Proof.
     intros; unfold ent_addr, addr2w.
     rewrite <- combine_nonzero_ok.
@@ -479,6 +488,13 @@ Definition avail xp cs :=
 
   Lemma vals_nonzero_addrs : forall l,
     length (vals_nonzero l) = nonzero_addrs (map fst l).
+  Proof.
+    induction l; intros; simpl; auto.
+    destruct a, n; simpl; auto.
+  Qed.
+
+  Lemma tags_nonzero_addrs : forall l,
+    length (tags_nonzero l) = nonzero_addrs (map fst l).
   Proof.
     induction l; intros; simpl; auto.
     destruct a, n; simpl; auto.
@@ -501,39 +517,44 @@ Definition avail xp cs :=
   Qed.
 
   Local Hint Resolve combine_nonzero_padded_wordToNat.
-
-  Lemma desc_padding_synced_piff : forall xp a l,
-    Desc.array_rep xp a (Desc.Synced (map ent_addr (padded_log l)))
-    <=p=> Desc.array_rep xp a (Desc.Synced (map ent_addr l)).
+  
+Lemma desc_padding_synced_piff : forall xp a l,
+    Desc.array_rep xp a (Desc.Synced (addr_tags (ndesc_log l)) (map ent_addr (padded_log l)))
+    <=p=> Desc.array_rep xp a (Desc.Synced (addr_tags (ndesc_log l)) (map ent_addr l)).
   Proof.
      unfold Desc.array_rep, Desc.synced_array, Desc.rep_common; intros.
      split; cancel; subst.
      unfold padded_log, setlen, roundup in H0.
      rewrite firstn_oob, map_app in H0 by auto.
      apply Desc.items_valid_app in H0; intuition.
-     apply eq_sym; apply desc_ipack_padded.
+     apply eq_sym.
+     rewrite  desc_ipack_padded; auto.
+     rewrite  <- desc_ipack_padded; auto.
      unfold padded_log, setlen, roundup.
      rewrite firstn_oob, map_app by auto.
      apply Desc.items_valid_app2; auto.
      autorewrite with lists; auto.
-     apply desc_ipack_padded.
+     rewrite <- desc_ipack_padded; auto.
+     rewrite <- desc_ipack_padded; auto.
   Qed.
 
   Lemma desc_padding_unsync_piff : forall xp a l,
-    Desc.array_rep xp a (Desc.Unsync (map ent_addr (padded_log l)))
-    <=p=> Desc.array_rep xp a (Desc.Unsync (map ent_addr l)).
+    Desc.array_rep xp a (Desc.Unsync (addr_tags (ndesc_log l)) (map ent_addr (padded_log l)))
+    <=p=> Desc.array_rep xp a (Desc.Unsync (addr_tags (ndesc_log l)) (map ent_addr l)).
   Proof.
      unfold Desc.array_rep, Desc.unsync_array, Desc.rep_common; intros.
      split; cancel; subst.
      unfold padded_log, setlen, roundup in H.
      rewrite firstn_oob, map_app in H by auto.
      apply Desc.items_valid_app in H; intuition.
-     apply eq_sym; apply desc_ipack_padded.
+     rewrite desc_ipack_padded; auto.
+     rewrite <- desc_ipack_padded; auto.
      unfold padded_log, setlen, roundup.
      rewrite firstn_oob, map_app by auto.
      apply Desc.items_valid_app2; auto.
      autorewrite with lists; auto.
-     apply desc_ipack_padded.
+     rewrite <- desc_ipack_padded; auto.
+     rewrite <- desc_ipack_padded; auto.
   Qed.
 
   Lemma goodSize_ndesc : forall l,
@@ -601,8 +622,16 @@ Definition avail xp cs :=
     rewrite IHa; auto.
   Qed.
 
+  Lemma tags_nonzero_app : forall a b,
+    tags_nonzero (a ++ b) = tags_nonzero a ++ tags_nonzero b.
+  Proof.
+    unfold tags_nonzero; induction a; intros; simpl; auto.
+    destruct a, n; simpl; auto.
+    rewrite IHa; auto.
+  Qed.
+
   Lemma log_nonzero_repeat_0 : forall n,
-    log_nonzero (repeat (0, $0) n) = nil.
+    log_nonzero (repeat (0, tagged_block0) n) = nil.
   Proof.
     induction n; simpl; auto.
   Qed.
@@ -619,6 +648,27 @@ Definition avail xp cs :=
     vals_nonzero (padded_log l) = vals_nonzero l.
   Proof.
     unfold vals_nonzero, padded_log, setlen, roundup; simpl.
+    induction l; intros; simpl; auto.
+    rewrite firstn_oob; simpl; auto.
+    rewrite log_nonzero_repeat_0; auto.
+
+    destruct a, n.
+    rewrite <- IHl.
+    repeat rewrite firstn_oob; simpl; auto.
+    repeat rewrite log_nonzero_app, map_app.
+    repeat rewrite log_nonzero_repeat_0; auto.
+
+    repeat rewrite firstn_oob; simpl; auto.
+    f_equal.
+    repeat rewrite log_nonzero_app, map_app.
+    repeat rewrite log_nonzero_repeat_0; auto.
+    simpl; rewrite app_nil_r; auto.
+  Qed.
+
+  Lemma tags_nonzero_padded_log : forall l,
+    tags_nonzero (padded_log l) = tags_nonzero l.
+  Proof.
+    unfold tags_nonzero, padded_log, setlen, roundup; simpl.
     induction l; intros; simpl; auto.
     rewrite firstn_oob; simpl; auto.
     rewrite log_nonzero_repeat_0; auto.
@@ -701,8 +751,1095 @@ Definition avail xp cs :=
   Arguments Desc.avail_rep : simpl never.
   Arguments Data.avail_rep : simpl never.
   Arguments divup : simpl never.
-  Hint Extern 0 (okToUnify (Hdr.rep _ _) (Hdr.rep _ _)) => constructor : okToUnify.
+  Hint Extern 0 (okToUnify (PermDiskLogHdr.rep _ _) (PermDiskLogHdr.rep _ _)) => constructor : okToUnify.
   Hint Extern 0 (okToUnify (Desc.array_rep _ _ _) (Desc.array_rep _ _ _)) => constructor : okToUnify.
   Hint Extern 0 (okToUnify (Data.array_rep _ _ _) (Data.array_rep _ _ _)) => constructor : okToUnify.
   Hint Extern 0 (okToUnify (Desc.avail_rep _ _ _) (Desc.avail_rep _ _ _)) => constructor : okToUnify.
   Hint Extern 0 (okToUnify (Data.avail_rep _ _ _) (Data.avail_rep _ _ _)) => constructor : okToUnify.
+
+
+  Definition avail_ok :
+    forall xp cs pr,
+    {< F l d,
+    PERM: pr                      
+    PRE:bm, hm,
+      PermCacheDef.rep cs d bm *
+      [[ (F * rep xp (Synced l) hm)%pred d ]]
+    POST:bm', hm', RET: ^(cs, r)
+          PermCacheDef.rep cs d bm' *
+          [[ (F * rep xp (Synced l) hm')%pred d ]] *
+          [[ r = (LogLen xp) - roundup (length l) DescSig.items_per_val ]]
+    CRASH:bm'', hm_crash, exists cs',
+          PermCacheDef.rep cs' d bm'' *
+          [[ (F * rep xp (Synced l) hm_crash)%pred d ]]
+    >} avail xp cs.
+  Proof.
+    unfold avail.
+    safestep.
+    safestep.
+    safestep.
+    solve_checksums.
+    eexists; repeat (eapply hashmap_subset_trans; eauto).
+    cancel; eauto.
+    rewrite <- H1; cancel.
+    solve_checksums.
+    eauto.
+  Qed.
+
+
+Theorem unseal_all_ok :
+    forall hl pr,
+    {!< F tbl,
+    PERM: pr                      
+    PRE:bm, hm,
+        F * [[ tbl = extract_blocks bm hl ]] *
+        [[ length tbl = length hl ]] *
+        [[ forall t, In t (map fst tbl) -> can_access pr t ]]
+    POST:bm', hm', RET: r
+        F * [[ r = map snd tbl ]]
+    CRASH:bm'', hm_crash,
+        false_pred (* Can't crash *)              
+    >!} unseal_all hl.
+  Proof.
+    unfold unseal_all; step.
+    safestep.
+    apply H3.
+    apply in_selN with (n:= m).
+    rewrite map_length.
+    setoid_rewrite H4; auto.
+    eassign (selN (map snd (extract_blocks bm hl)) m ($0)).
+    erewrite extract_blocks_selN.
+    repeat erewrite selN_map.
+    rewrite <- surjective_pairing; auto.
+    unfold block_mem_subset in *.
+
+    erewrite extract_blocks_subset with (bm:= bm); eauto.
+    setoid_rewrite H4; omega.
+    setoid_rewrite H4; omega.
+    erewrite <- extract_blocks_subset with (bm:= bm); eauto.
+    auto.
+
+    step.
+    step.
+    rewrite H11.
+    replace ([(map snd (extract_blocks bm hl)) ⟦ m ⟧]) with
+        (map snd [selN (extract_blocks bm hl) m tagged_block0]).
+    rewrite <- map_app.
+    erewrite <- extract_blocks_subset with (bm:= bm); eauto.
+    erewrite extract_blocks_selN_inside; auto.
+    rewrite <- extract_blocks_app.
+    rewrite <- firstn_S_selN; auto.
+    erewrite extract_blocks_subset with (bm:= bm); eauto.
+
+    erewrite extract_blocks_firstn_length; auto.
+    erewrite extract_blocks_firstn_length; auto.
+    simpl; erewrite selN_map; auto.
+    setoid_rewrite H4; omega.
+    eexists; repeat (eapply hashmap_subset_trans; eauto).
+    cancel; eauto.
+
+    step.
+    step.
+    rewrite H9, firstn_exact.
+    erewrite extract_blocks_subset with (bm:= bm); eauto.
+    eexists; repeat (eapply hashmap_subset_trans; eauto).
+    eassign (lift_empty(False) (AT:= addr)(AEQ:=addr_eq_dec)(V:=valuset))%pred; cancel.
+    Unshelve.
+    all: eauto.
+    exact tt.
+    exact Public.
+    exact tagged_block0.
+  Qed.
+
+
+  Hint Extern 1 ({{_|_}} Bind (unseal_all _) _) => apply unseal_all_ok : prog.
+
+
+
+  Lemma combine_tags_vals:
+    forall l,
+      combine (tags_nonzero l) (Data.Defs.ipack (vals_nonzero l)) = blocks_nonzero l.
+  Proof.
+    induction l; simpl; intuition.
+    destruct a, n, t; auto.
+    unfold Data.Defs.ipack in *.
+    unfold Data.Defs.list_chunk, DataSig.items_per_val in *.
+    rewrite divup_1 in *.
+    simpl.
+    rewrite setlen_inbound; simpl.
+    unfold tags_nonzero, blocks_nonzero, vals_nonzero in *; simpl.
+    setoid_rewrite IHl.
+    unfold ent_tag, ent_valu; simpl.
+    admit.
+    omega.
+  Admitted.
+
+  
+
+  Definition read_ok :
+    forall xp cs pr,
+    {< F l d,
+    PERM: pr                      
+    PRE:bm, hm,
+          PermCacheDef.rep cs d bm *
+          [[ (F * rep xp (Synced l) hm)%pred d ]]
+    POST:bm', hm', RET: ^(cs, r)
+          PermCacheDef.rep cs d bm' *
+          [[ (F * rep xp (Synced l) hm')%pred d ]] *
+          [[ combine_nonzero (fst r) (extract_blocks bm' (snd r)) = log_nonzero l ]]
+    CRASH:bm'', hm_crash, exists cs',
+          PermCacheDef.rep cs' d bm'' *
+          [[ (F * rep xp (Synced l) hm_crash)%pred d ]]
+    >} read xp cs.
+  Proof.
+    unfold read.
+    safestep.
+
+    prestep. norm. cancel. intuition simpl.
+    eassign (map ent_addr (padded_log l)).
+    rewrite map_length, padded_log_length.
+    auto.
+    eassign (addr_tags (ndesc_log l)).
+    unfold addr_tags; apply repeat_length.
+    auto.
+    pred_apply.
+    rewrite desc_padding_synced_piff; cancel.
+    subst.
+
+    step.
+    rewrite H18, H19; auto.
+    rewrite H19 in H8.
+    apply in_map_fst_exists_snd in H8; cleanup.
+    apply in_combine_l in H8.
+    unfold addr_tags in H8.
+    apply repeat_spec in H8; subst; auto.
+
+    safestep; subst.
+    erewrite block_mem_subset_rep; eauto.
+    eassign (vals_nonzero l).
+    setoid_rewrite vals_nonzero_addrs; unfold ndata_log.
+    replace DataSig.items_per_val with 1 by (cbv; auto); try omega.
+    eassign (tags_nonzero l).
+    setoid_rewrite tags_nonzero_addrs; unfold ndata_log.
+    replace DataSig.items_per_val with 1 by (cbv; auto); try omega.
+    pred_apply; cancel.
+    auto.
+    
+    safestep.
+    safestep.
+    rewrite desc_padding_synced_piff; cancel.
+    solve_checksums.
+
+    subst.
+    rewrite H19, H26.
+    rewrite map_snd_combine.
+    erewrite DescDefs.iunpack_ipack; eauto.
+
+    rewrite combine_tags_vals.
+    apply combine_nonzero_padded_wordToNat; auto.
+    rewrite map_length.
+    rewrite padded_log_length.
+    unfold roundup; eauto.
+    unfold addr_tags; rewrite repeat_length.
+    unfold ndesc_log.
+    rewrite Desc.Defs.ipack_length.
+    rewrite map_length.
+    rewrite padded_log_length.
+    unfold roundup; rewrite divup_mul; auto.
+    unfold DescSig.items_per_val.
+    rewrite valulen_is. cbv; omega.
+    eexists; repeat (eapply hashmap_subset_trans; eauto).
+    unfold pimpl; intros; eapply block_mem_subset_trans; eauto.
+
+    cancel; eauto.
+    rewrite <- H1; cancel.
+    rewrite desc_padding_synced_piff; cancel.
+    solve_checksums.
+    eexists; repeat (eapply hashmap_subset_trans; eauto).
+    unfold pimpl; intros; eapply block_mem_subset_trans; eauto.
+
+    rewrite <- H1; cancel.
+    solve_checksums.
+    eexists; repeat (eapply hashmap_subset_trans; eauto).
+    unfold pimpl; intros; eapply block_mem_subset_trans; eauto.
+
+    rewrite <- H1; cancel.
+    solve_checksums.
+    eexists; repeat (eapply hashmap_subset_trans; eauto).
+
+    Unshelve.
+    all: unfold EqDec; apply handle_eq_dec.
+  Qed.
+
+
+
+  Lemma goodSize_0 : forall sz, goodSize sz 0.
+  Proof.
+    unfold goodSize; intros.
+    apply zero_lt_pow2.
+  Qed.
+
+  Lemma ndesc_log_nil : ndesc_log nil = 0.
+  Proof.
+    unfold ndesc_log; simpl.
+    rewrite divup_0; auto.
+  Qed.
+
+  Lemma ndata_log_nil : ndata_log nil = 0.
+  Proof.
+    unfold ndata_log; simpl; auto.
+  Qed.
+
+  Local Hint Resolve goodSize_0.
+
+
+  Definition init xp cs :=
+    cs <- PermDiskLogHdr.init xp cs;;
+    Ret cs.
+
+  Definition trunc xp cs :=
+    let^ (cs, nr) <- PermDiskLogHdr.read xp cs;;
+    let '(_, current_length, _) := nr in
+    h <- Hash default_encoding;; 
+    cs <- PermDiskLogHdr.write xp (current_length, (0, 0), (h, h)) cs;;
+    cs <- PermDiskLogHdr.sync_now xp cs;;
+    Ret cs.
+
+  Local Hint Resolve Forall_nil.
+
+
+  Definition initrep xp :=
+    (exists hdr, LogHeader xp |+> hdr *
+     Desc.avail_rep xp 0 (LogDescLen xp) *
+     Data.avail_rep xp 0 (LogLen xp))%pred.
+
+
+  Definition init_ok' :
+    forall xp cs pr,
+    {< F d,
+    PERM: pr   
+    PRE:bm, hm,
+      PermCacheDef.rep cs d bm *
+      [[ (F * initrep xp)%pred d ]] *
+      [[ xparams_ok xp /\ sync_invariant F ]]
+    POST:bm', hm', RET: cs  exists d',
+          PermCacheDef.rep cs d' bm' *
+          [[ (F * rep xp (Synced nil) hm')%pred d' ]]
+    XCRASH:bm'', hm_crash, any
+    >} init xp cs.
+  Proof.
+    unfold init, initrep.
+    prestep; unfold rep, PermDiskLogHdr.LAHdr; safecancel.
+    eassign (t,l); cancel.
+    auto.
+    step.
+    step.
+    unfold ndesc_log, ndata_log; rewrite divup_0; simpl; cancel.
+    repeat rewrite Nat.sub_0_r; cbn; cancel.
+    rewrite Desc.array_rep_sync_nil, Data.array_rep_sync_nil by (auto; omega); cancel.
+    solve_checksums; simpl; auto.
+    setoid_rewrite DescDefs.ipack_nil; simpl.
+    unfold ndesc_log, addr_tags; rewrite divup_0; simpl.
+    solve_hash_list_rep; auto.
+    eexists; repeat (eapply hashmap_subset_trans; eauto).
+  Qed.
+
+  Definition init_ok :
+    forall xp cs pr,
+    {< F l d,
+    PERM: pr
+    PRE:bm, hm,
+      PermCacheDef.rep cs d bm *
+      [[ (F * arrayS (LogHeader xp) l)%pred d ]] *
+      [[ length l = (1 + LogDescLen xp + LogLen xp) /\
+         LogDescriptor xp = LogHeader xp + 1 /\
+         LogData xp = LogDescriptor xp + LogDescLen xp /\
+         xparams_ok xp ]] *
+      [[ sync_invariant F ]]
+    POST:bm', hm', RET: cs  exists d',
+      PermCacheDef.rep cs d' bm' *
+      [[ (F * rep xp (Synced nil) hm')%pred d' ]]
+    XCRASH:bm'', hm_crash, any
+    >} init xp cs.
+  Proof.
+    intros.
+    eapply pimpl_ok2. apply init_ok'.
+    intros; unfold initrep; safecancel.
+    unfold Desc.avail_rep, Data.avail_rep.
+    rewrite arrayN_isolate_hd by omega.
+    repeat rewrite Nat.add_0_r.
+    rewrite arrayN_split with (i := LogDescLen xp).
+    rewrite surjective_pairing with (p := selN l 0 valuset0).
+    substl (LogData xp); substl (LogDescriptor xp).
+    cancel.
+    eassign F; cancel.
+    rewrite firstn_length_l; auto.
+    setoid_rewrite skipn_length with (n := 1); omega.
+    setoid_rewrite skipn_skipn with (m := 1).
+    rewrite skipn_length; omega.
+    auto.
+    step.
+  Qed.
+
+  Hint Extern 1 ({{_|_}} Bind (init _ _) _) => apply init_ok : prog.
+
+   Lemma helper_sep_star_reorder : forall (a b c d : rawpred),
+    a * b * c * d =p=> (a * c) * (b * d).
+  Proof.
+    intros; cancel.
+  Qed.
+
+  Lemma helper_add_sub_0 : forall a b,
+    a <= b -> a + (b - a) + 0 = b.
+  Proof.
+    intros; omega.
+  Qed.
+
+  Lemma helper_trunc_ok : forall xp l prev_len h,
+    Desc.array_rep xp 0 (Desc.Synced (addr_tags (ndesc_log l)) (map ent_addr l)) *
+    Data.array_rep xp 0 (Data.Synced (tags_nonzero l) (vals_nonzero l)) *
+    Desc.avail_rep xp (ndesc_log l) (LogDescLen xp - ndesc_log l) *
+    Data.avail_rep xp (ndata_log l) (LogLen xp - ndata_log l) *
+    PermDiskLogHdr.rep xp (PermDiskLogHdr.Synced (prev_len, (0, 0), h))
+    =p=>
+    PermDiskLogHdr.rep xp (PermDiskLogHdr.Synced (prev_len, (ndesc_log [], ndata_log []), h)) *
+    Desc.array_rep xp 0 (Desc.Synced (addr_tags (ndesc_log [])) []) *
+    Data.array_rep xp 0 (Data.Synced (tags_nonzero []) (vals_nonzero [])) *
+    Desc.avail_rep xp (ndesc_log []) (LogDescLen xp - ndesc_log []) *
+    Data.avail_rep xp (ndata_log []) (LogLen xp - ndata_log []).
+  Proof.
+    intros.
+    unfold ndesc_log, tags_nonzero, vals_nonzero; simpl; rewrite divup_0.
+    rewrite Desc.array_rep_sync_nil_sep_star, Data.array_rep_sync_nil_sep_star; auto.
+    cancel.
+    unfold ndata_log; simpl; repeat rewrite Nat.sub_0_r.
+    rewrite <- log_nonzero_addrs.
+    rewrite Data.array_rep_size_ok_pimpl, Desc.array_rep_size_ok_pimpl.
+    rewrite Data.array_rep_avail, Desc.array_rep_avail.
+    simpl; rewrite divup_1; autorewrite with lists.
+    cancel.
+    rewrite helper_sep_star_reorder.
+    rewrite Desc.avail_rep_merge by auto.
+    rewrite Data.avail_rep_merge by auto.
+    repeat rewrite helper_add_sub_0 by auto.
+    cancel.
+  Qed.
+
+
+  (* XXX:
+    Ideally XCRASH can contain only Truncated state, whose crash_xform 
+    covers the Synced state's crash_xform. However, to prove that, we need 
+    to construct a raw disk that satisifies the Truncated state given a raw
+    disk of Synced state.  This involves reverse engineering Hdr.rep.
+  *)
+  Definition trunc_ok :
+    forall xp cs pr,
+    {< F l d,
+    PERM: pr                       
+    PRE:bm, hm,
+     PermCacheDef.rep cs d bm *
+     [[ (F * rep xp (Synced l) hm)%pred d ]] *
+     [[ sync_invariant F ]]
+    POST:bm', hm', RET: cs  exists d',
+     PermCacheDef.rep cs d' bm' *
+     [[ (F * rep xp (Synced nil) hm')%pred d' ]]
+    XCRASH:bm'', hm_crash, exists cs' d',
+     PermCacheDef.rep cs' d' bm'' * (
+       [[ (F * (rep xp (Synced l) hm_crash))%pred d' ]] \/
+       [[ (F * (rep xp (Truncated l) hm_crash))%pred d' ]] )
+    >} trunc xp cs.
+  Proof.
+    unfold trunc.
+    step.
+    step.
+    step.
+
+    unfold PermDiskLogHdr.rep in H0.
+    destruct_lift H0.
+    unfold hdr_goodSize in *; intuition.
+
+    step.
+    step.
+    step.
+
+    (* post condition *)
+    cancel_by helper_trunc_ok.
+    solve_checksums.
+    replace (DescDefs.ipack (map ent_addr [])) with (@nil valu).
+    unfold ndesc_log, addr_tags; rewrite divup_0; simpl.
+    solve_hash_list_rep; auto.
+    symmetry. apply DescDefs.ipack_nil.
+    auto.
+    eexists; repeat (eapply hashmap_subset_trans; eauto).
+
+    (* crash conditions *)
+    rewrite <- H1; cancel.
+    eexists; repeat (eapply hashmap_subset_trans; eauto).
+    unfold pimpl; intros; eapply block_mem_subset_trans; eauto.
+    
+    xform_norm. cancel. xform_normr; cancel.
+    eassign cs'; eassign d'; cancel.
+    or_r; cancel.
+    solve_checksums.
+    solve_checksums; auto.
+    setoid_rewrite DescDefs.ipack_nil; simpl.
+    unfold ndesc_log, addr_tags; rewrite divup_0; simpl.
+    solve_hash_list_rep; auto.
+
+    rewrite <- H1; cancel.
+    eexists; repeat (eapply hashmap_subset_trans; eauto).
+    unfold pimpl; intros; eapply block_mem_subset_trans; eauto.
+    repeat xcrash_rewrite.
+    xform_norm; cancel. xform_normr; cancel.
+    eassign x; eassign x0; cancel.
+    or_r; cancel.
+    solve_checksums.
+    solve_checksums; auto.
+    setoid_rewrite DescDefs.ipack_nil; simpl.
+    unfold ndesc_log, addr_tags; rewrite divup_0; simpl.
+    solve_hash_list_rep; auto.
+
+    rewrite <- H1; cancel.
+    eexists; repeat (eapply hashmap_subset_trans; eauto).     
+    xform_normr; cancel.
+    eassign cs'; eassign d; cancel.
+    or_l; cancel.
+    solve_checksums.
+
+    Unshelve.
+    all: unfold EqDec; apply handle_eq_dec.
+  Qed.
+
+
+
+  Theorem loglen_valid_dec xp ndesc ndata :
+    {loglen_valid xp ndesc ndata} + {loglen_invalid xp ndesc ndata }.
+  Proof.
+    unfold loglen_valid, loglen_invalid.
+    destruct (lt_dec (LogDescLen xp) ndesc);
+    destruct (lt_dec (LogLen xp) ndata); simpl; auto.
+    left; intuition.
+  Defined.
+
+  Remove Hints goodSize_0.
+
+  Definition entry_valid_ndata : forall l,
+    Forall entry_valid l -> ndata_log l = length l.
+  Proof.
+    unfold ndata_log; induction l; rewrite Forall_forall; intuition.
+    destruct a, n; simpl.
+    exfalso; intuition.
+    apply (H (0, t)); simpl; auto.
+    rewrite IHl; auto.
+    rewrite Forall_forall; intros.
+    apply H; simpl; intuition.
+  Qed.
+
+  Lemma loglen_valid_desc_valid : forall xp old new,
+    DescSig.xparams_ok xp ->
+    loglen_valid xp (ndesc_log old + ndesc_log new) (ndata_log old + ndata_log new) ->
+    Desc.items_valid xp (ndesc_log old) (map ent_addr new).
+  Proof.
+    unfold Desc.items_valid, loglen_valid.
+    intuition.
+    unfold DescSig.RALen; omega.
+    autorewrite with lists; unfold DescSig.RALen.
+    apply divup_ge; auto.
+    unfold ndesc_log in *; omega.
+  Qed.
+  Local Hint Resolve loglen_valid_desc_valid.
+
+
+  Lemma loglen_valid_data_valid : forall xp old new,
+    DataSig.xparams_ok xp ->
+    Forall entry_valid new ->
+    loglen_valid xp (ndesc_log old + ndesc_log new) (ndata_log old + ndata_log new) ->
+    Data.items_valid xp (ndata_log old) (map ent_valu new).
+  Proof.
+    unfold Data.items_valid, loglen_valid.
+    intuition.
+    unfold DataSig.RALen; omega.
+    autorewrite with lists; unfold DataSig.RALen.
+    apply divup_ge; auto.
+    rewrite divup_1; rewrite <- entry_valid_ndata by auto.
+    unfold ndata_log in *; omega.
+  Qed.
+  Local Hint Resolve loglen_valid_data_valid.
+
+  Lemma helper_loglen_desc_valid_extend : forall xp new old,
+    loglen_valid xp (ndesc_log old + ndesc_log new) (ndata_log old + ndata_log new) ->
+    ndesc_log new + (LogDescLen xp - ndesc_log old - ndesc_log new) 
+      = LogDescLen xp - ndesc_log old.
+  Proof.
+    unfold loglen_valid, ndesc_log; intros.
+    omega.
+  Qed.
+
+  Lemma helper_loglen_data_valid_extend : forall xp new old,
+    loglen_valid xp (ndesc_log old + ndesc_log new) (ndata_log old + ndata_log new) ->
+    ndata_log new + (LogLen xp - ndata_log old - ndata_log new) 
+      = LogLen xp - ndata_log old.
+  Proof.
+    unfold loglen_valid, ndata_log; intros.
+    omega.
+  Qed.
+
+  Lemma helper_loglen_data_valid_extend_entry_valid : forall xp new old,
+    Forall entry_valid new ->
+    loglen_valid xp (ndesc_log old + ndesc_log new) (ndata_log old + ndata_log new) ->
+    length new + (LogLen xp - ndata_log old - ndata_log new) 
+      = LogLen xp - ndata_log old.
+  Proof.
+    intros.
+    rewrite <- entry_valid_ndata by auto.
+    apply helper_loglen_data_valid_extend; auto.
+  Qed.
+
+  Lemma padded_desc_valid : forall xp st l,
+    Desc.items_valid xp st (map ent_addr l)
+    -> Desc.items_valid xp st (map ent_addr (padded_log l)).
+  Proof.
+    unfold Desc.items_valid; intuition.
+    autorewrite with lists in *.
+    rewrite padded_log_length; unfold roundup.
+    apply Nat.mul_le_mono_pos_r.
+    apply DescDefs.items_per_val_gt_0.
+    apply divup_le; lia.
+  Qed.
+
+  Lemma mul_le_mono_helper : forall a b,
+    b > 0 -> a <= a * b.
+  Proof.
+    intros; rewrite Nat.mul_comm.
+    destruct (mult_O_le a b); auto; omega.
+  Qed.
+
+  Lemma loglen_valid_goodSize_l : forall xp a b,
+    loglen_valid xp a b -> DescSig.xparams_ok xp -> DataSig.xparams_ok xp ->
+    goodSize addrlen a.
+  Proof.
+    unfold loglen_valid, DescSig.xparams_ok, DataSig.xparams_ok; intuition.
+    eapply goodSize_trans.
+    eapply le_trans. eauto.
+    apply le_plus_r. eauto.
+  Qed.
+
+  Lemma loglen_valid_goodSize_r : forall xp a b,
+    loglen_valid xp a b -> DescSig.xparams_ok xp -> DataSig.xparams_ok xp ->
+    goodSize addrlen b.
+  Proof.
+    unfold loglen_valid, DescSig.xparams_ok, DataSig.xparams_ok; intuition.
+    eapply goodSize_trans.
+    eapply le_trans. eauto.
+    apply le_plus_r. eauto.
+  Qed.
+
+  Lemma ent_valid_addr_valid : forall l,
+    Forall entry_valid l -> Forall addr_valid l.
+  Proof.
+    intros; rewrite Forall_forall in *; intros.
+    apply H; auto.
+  Qed.
+  Local Hint Resolve ent_valid_addr_valid.
+  Local Hint Resolve Forall_append DescDefs.items_per_val_not_0.
+
+  Lemma helper_add_sub : forall a b,
+    a <= b -> a + (b - a) = b.
+  Proof.
+    intros; omega.
+  Qed.
+
+
+  Lemma nonzero_addrs_app : forall a b,
+    nonzero_addrs (a ++ b) = nonzero_addrs a + nonzero_addrs b.
+  Proof.
+    induction a; intros; simpl; auto.
+    destruct a; auto.
+    rewrite IHa; omega.
+  Qed.
+
+  Lemma ndata_log_app : forall a b,
+    ndata_log (a ++ b) = ndata_log a + ndata_log b.
+  Proof.
+    unfold ndata_log;  intros.
+    repeat rewrite map_app.
+    rewrite nonzero_addrs_app; auto.
+  Qed.
+
+  Lemma ndesc_log_padded_log : forall l,
+    ndesc_log (padded_log l) = ndesc_log l.
+  Proof.
+    unfold ndesc_log; intros.
+    rewrite padded_log_length.
+    unfold roundup; rewrite divup_divup; auto.
+  Qed.
+
+  Lemma ndesc_log_app : forall a b,
+    length a = roundup (length a) DescSig.items_per_val ->
+    ndesc_log (a ++ b) = ndesc_log a + ndesc_log b.
+  Proof.
+    unfold ndesc_log; intros.
+    rewrite app_length, H at 1.
+    unfold roundup.
+    rewrite Nat.add_comm, Nat.mul_comm.
+    rewrite divup_add by auto.
+    omega.
+  Qed.
+
+  Lemma ndesc_log_padded_app : forall a b,
+    ndesc_log (padded_log a ++ b) = ndesc_log a + ndesc_log b.
+  Proof.
+    intros.
+    rewrite ndesc_log_app.
+    rewrite ndesc_log_padded_log; auto.
+    rewrite padded_log_length.
+    rewrite roundup_roundup; auto.
+  Qed.
+
+  Lemma ndata_log_padded_log : forall a,
+    ndata_log (padded_log a) = ndata_log a.
+  Proof.
+    unfold ndata_log, padded_log, setlen, roundup; intros.
+    rewrite firstn_oob by auto.
+    repeat rewrite map_app.
+    rewrite repeat_map; simpl.
+    rewrite nonzero_addrs_app.
+    setoid_rewrite <- app_nil_l at 3.
+    rewrite nonzero_addrs_app_zeros; auto.
+  Qed.
+
+
+  Lemma ndata_log_padded_app : forall a b,
+    ndata_log (padded_log a ++ b) = ndata_log a + ndata_log b.
+  Proof.
+    intros.
+    rewrite ndata_log_app.
+    rewrite ndata_log_padded_log; auto.
+  Qed.
+
+  Lemma log_nonzero_rev_comm : forall l,
+    log_nonzero (rev l) = rev (log_nonzero l).
+  Proof.
+    induction l; simpl; intros; auto.
+    destruct a, n; simpl; auto;
+    rewrite log_nonzero_app; simpl.
+    rewrite app_nil_r. congruence.
+    congruence.
+  Qed.
+
+  Lemma entry_valid_vals_nonzero : forall l,
+    Forall entry_valid l ->
+    log_nonzero l = l.
+  Proof.
+    unfold entry_valid; induction l; simpl; auto.
+    destruct a, n; simpl; auto; intros.
+    exfalso.
+    rewrite Forall_forall in H; intuition.
+    apply (H (0, t)); simpl; auto.
+    rewrite IHl; auto.
+    eapply Forall_cons2; eauto.
+  Qed.
+
+  Lemma nonzero_addrs_entry_valid : forall l,
+    Forall entry_valid l ->
+    nonzero_addrs (map fst l) = length l.
+  Proof.
+    induction l; simpl; intros; auto.
+    destruct a, n; simpl.
+    exfalso.
+    rewrite Forall_forall in H.
+    apply (H (0, t)); simpl; auto.
+    rewrite IHl; auto.
+    eapply Forall_cons2; eauto.
+  Qed.
+
+  Lemma desc_ipack_injective : forall l1 l2 n1 n2,
+    length l1 = n1 * DescSig.items_per_val ->
+    length l2 = n2 * DescSig.items_per_val ->
+    DescDefs.ipack l1 = DescDefs.ipack l2 ->
+    l1 = l2.
+  Proof.
+    intros.
+    erewrite <- DescDefs.iunpack_ipack; eauto.
+    erewrite <- DescDefs.iunpack_ipack at 1; eauto.
+    congruence.
+  Qed.
+
+  Lemma ndesc_log_ndesc_list : forall l,
+    ndesc_log l = ndesc_list (map ent_addr (padded_log l)).
+  Proof.
+    unfold ndesc_log, ndesc_list.
+    intros.
+    autorewrite with lists.
+    rewrite padded_log_length.
+    unfold roundup.
+    rewrite divup_divup; auto.
+  Qed.
+
+  Lemma addr_tags_app:
+    forall n m,
+      addr_tags (n + m) = addr_tags n ++ addr_tags m.
+  Proof.
+    induction n; simpl; intros; auto.
+    unfold addr_tags in *; simpl; auto.
+    rewrite IHn; auto.
+  Qed.
+  
+  Lemma extend_ok_helper : forall F xp old new,
+    Forall entry_valid new ->
+    Data.array_rep xp (ndata_log old) (Data.Synced (map ent_tag new) (map ent_valu new)) *
+    Desc.array_rep xp 0 (Desc.Synced (addr_tags (ndesc_log old)) (map ent_addr old)) *
+    Data.array_rep xp 0 (Data.Synced (tags_nonzero old) (vals_nonzero old)) *
+    Desc.avail_rep xp (ndesc_log old + divup (length (map ent_addr new)) DescSig.items_per_val)
+      (LogDescLen xp - ndesc_log old - ndesc_log new) *
+    Data.avail_rep xp (ndata_log old + divup (length (map ent_valu new)) DataSig.items_per_val)
+      (LogLen xp - ndata_log old - ndata_log new) *
+    Desc.array_rep xp (ndesc_log old) (Desc.Synced (addr_tags (ndesc_log new)) (map ent_addr (padded_log new))) * F
+    =p=>
+    Desc.array_rep xp 0 (Desc.Synced (addr_tags (ndesc_log (padded_log old ++ new))) (map ent_addr (padded_log old ++ new))) *
+    Data.array_rep xp 0 (Data.Synced (tags_nonzero (padded_log old ++ new)) (vals_nonzero (padded_log old ++ new))) *
+    Desc.avail_rep xp (ndesc_log (padded_log old ++ new)) 
+                      (LogDescLen xp - ndesc_log (padded_log old ++ new)) *
+    Data.avail_rep xp (ndata_log (padded_log old ++ new))
+                      (LogLen xp - ndata_log (padded_log old ++ new)) * F.
+  Proof.
+    intros.
+    repeat rewrite ndesc_log_padded_app, ndata_log_padded_app.
+    setoid_rewrite Nat.sub_add_distr.
+    (* unfold ndesc_log. *)
+    rewrite divup_1.
+    rewrite entry_valid_ndata with (l := new); auto.
+    repeat rewrite map_length.
+    rewrite map_app, vals_nonzero_app.
+    rewrite addr_tags_app.
+    rewrite <- Desc.array_rep_synced_app.
+    rewrite tags_nonzero_app.
+    rewrite <- Data.array_rep_synced_app.
+    repeat rewrite Nat.add_0_l.
+    repeat rewrite desc_padding_synced_piff.
+    repeat rewrite map_length.
+    repeat rewrite vals_nonzero_padded_log, tags_nonzero_padded_log.
+    repeat rewrite divup_1, padded_log_length.
+    unfold roundup; rewrite divup_mul; auto.
+    unfold ndata_log; rewrite vals_nonzero_addrs.
+    unfold tags_nonzero, vals_nonzero; rewrite entry_valid_vals_nonzero with (l := new); auto.
+    cancel.
+
+    rewrite Nat.mul_1_r; auto.
+    rewrite map_length, padded_log_length.
+    unfold roundup; auto.
+  Qed.
+
+  Lemma nonzero_addrs_bound : forall l,
+    nonzero_addrs l <= length l.
+  Proof.
+    induction l; simpl; auto.
+    destruct a; omega.
+  Qed.
+
+  Lemma extend_ok_synced_hdr_helper : forall xp prev_len old new h,
+    PermDiskLogHdr.rep xp (PermDiskLogHdr.Synced (prev_len,
+                            (ndesc_log old + ndesc_log new,
+                             ndata_log old + ndata_log new),
+                            h))
+    =p=>
+    PermDiskLogHdr.rep xp (PermDiskLogHdr.Synced (prev_len,
+                            (ndesc_log (padded_log old ++ new),
+                             ndata_log (padded_log old ++ new)),
+                            h)).
+  Proof.
+    intros.
+    rewrite ndesc_log_padded_app, ndata_log_padded_app; auto.
+  Qed.
+
+  Local Hint Resolve extend_ok_synced_hdr_helper.
+
+  Lemma nonzero_addrs_roundup : forall B (l : list (addr * B)) n,
+    n > 0 ->
+    nonzero_addrs (map fst l) <= (divup (length l) n) * n.
+  Proof.
+    intros.
+    eapply le_trans.
+    apply nonzero_addrs_bound.
+    rewrite map_length.
+    apply roundup_ge; auto.
+  Qed.
+
+  Lemma loglen_invalid_overflow : forall xp old new,
+    LogLen xp = DescSig.items_per_val * LogDescLen xp ->
+    loglen_invalid xp (ndesc_log old + ndesc_log new) (ndata_log old + ndata_log new) ->
+    length (padded_log old ++ new) > LogLen xp.
+  Proof.
+    unfold loglen_invalid, ndesc_log, ndata_log; intros.
+    rewrite app_length; repeat rewrite padded_log_length.
+    unfold roundup; intuition.
+    rewrite H.
+    setoid_rewrite <- Nat.mul_comm at 2.
+    apply divup_add_gt; auto.
+
+    eapply lt_le_trans; eauto.
+    apply Nat.add_le_mono.
+    apply nonzero_addrs_roundup; auto.
+    erewrite <- map_length.
+    apply nonzero_addrs_bound.
+  Qed.
+
+  Hint Rewrite Desc.array_rep_avail Data.array_rep_avail
+     padded_log_length divup_mul divup_1 map_length
+     ndesc_log_padded_log nonzero_addrs_padded_log using auto: extend_crash.
+  Hint Unfold roundup ndata_log : extend_crash.
+
+  Ltac extend_crash :=
+     repeat (autorewrite with extend_crash; autounfold with extend_crash; simpl);
+     setoid_rewrite <- Desc.avail_rep_merge at 3;
+     [ setoid_rewrite <- Data.avail_rep_merge at 3 | ];
+     [ cancel
+     | apply helper_loglen_data_valid_extend_entry_valid; auto
+     | apply helper_loglen_desc_valid_extend; auto ].
+
+  Lemma log_nonzero_padded_log : forall l,
+    log_nonzero (padded_log l) = log_nonzero l.
+  Proof.
+    unfold padded_log, setlen, roundup; intros.
+    rewrite firstn_oob by auto.
+    rewrite log_nonzero_app.
+    rewrite log_nonzero_repeat_0, app_nil_r; auto.
+  Qed.
+
+  Lemma log_nonzero_padded_app : forall l new,
+    Forall entry_valid new ->
+    log_nonzero l ++ new = log_nonzero (padded_log l ++ padded_log new).
+  Proof.
+    intros.
+    rewrite log_nonzero_app.
+    repeat rewrite log_nonzero_padded_log.
+    f_equal.
+    rewrite entry_valid_vals_nonzero; auto.
+  Qed.
+
+  Lemma log_nonzero_app_padded : forall l new,
+    Forall entry_valid new ->
+    log_nonzero l ++ new = log_nonzero (l ++ padded_log new).
+  Proof.
+    intros.
+    rewrite log_nonzero_app, log_nonzero_padded_log.
+    f_equal.
+    rewrite entry_valid_vals_nonzero; auto.
+  Qed.
+
+
+
+
+(* Need to add If statement and alighned functions *)
+
+  
+
+  Definition extend xp log cs :=
+    (* Synced *)
+    let^ (cs, nr) <- PermDiskLogHdr.read xp cs;;
+    let '(_, (ndesc, ndata), (h_addr, h_valu)) := nr in
+    let '(nndesc, nndata) := ((ndesc_log log), (ndata_log log)) in
+    If (loglen_valid_dec xp (ndesc + nndesc) (ndata + nndata)) {
+      h_addr <- hash_list h_addr (DescDefs.nopad_ipack (map ent_addr log));
+      h_valu <- hash_list h_valu (vals_nonzero log);
+      cs <- Desc.write_aligned xp ndesc (map ent_addr log) cs;
+      cs <- Data.write_aligned xp ndata (map ent_valu log) cs;
+      cs <- Hdr.write xp ((ndesc, ndata),
+                          (ndesc + nndesc, ndata + nndata),
+                          (h_addr, h_valu)) cs;
+      (* Extended *)
+      cs <- BUFCACHE.begin_sync cs;
+      cs <- Desc.sync_aligned xp ndesc nndesc cs;
+      cs <- Data.sync_aligned xp ndata nndata cs;
+      cs <- Hdr.sync xp cs;
+      cs <- BUFCACHE.end_sync cs;
+      (* Synced *)
+      Ret ^(cs, true)
+    } else {
+      Ret ^(cs, false)
+    }.
+
+  Lemma rep_hashmap_subset : forall xp hm hm',
+    (exists l, hashmap_subset l hm hm')
+    -> forall st, rep xp st hm
+        =p=> rep xp st hm'.
+  Proof.
+    intros.
+    destruct st; unfold rep, rep_inner; cancel; solve_checksums.
+    auto.
+  Qed.
+
+  Lemma would_recover'_hashmap_subset : forall xp l hm hm',
+    (exists l, hashmap_subset l hm hm') ->
+    would_recover' xp l hm
+    =p=> would_recover' xp l hm'.
+  Proof.
+    unfold would_recover'.
+    intros.
+    cancel;
+    rewrite rep_hashmap_subset; auto; cancel.
+  Qed.
+
+  Definition extend_ok : forall xp new cs,
+    {< F old d,
+    PRE:hm   BUFCACHE.rep cs d *
+          [[ (F * rep xp (Synced old) hm)%pred d ]] *
+          [[ Forall entry_valid new /\ sync_invariant F ]]
+    POST:hm' RET: ^(cs, r) exists d',
+          BUFCACHE.rep cs d' * (
+          [[ r = true /\
+             (F * rep xp (Synced ((padded_log old) ++ new)) hm')%pred d' ]] \/
+          [[ r = false /\ length ((padded_log old) ++ new) > LogLen xp /\
+             (F * rep xp (Synced old) hm')%pred d' ]])
+    XCRASH:hm_crash exists cs' d',
+          BUFCACHE.rep cs' d' * (
+          [[ (F * rep xp (Synced old) hm_crash)%pred d' ]] \/
+          [[ (F * rep xp (Extended old new) hm_crash)%pred d' ]])
+    >} extend xp new cs.
+  Proof.
+    unfold extend.
+    step.
+    step.
+
+    (* true case *)
+    - (* write content *)
+      rewrite <- DescDefs.ipack_nopad_ipack_eq.
+      step.
+      unfold checksums_match in *; intuition.
+      solve_hash_list_rep.
+      step.
+      unfold checksums_match in *; intuition.
+      solve_hash_list_rep.
+
+      safestep.
+      rewrite Desc.avail_rep_split. cancel.
+      autorewrite with lists; apply helper_loglen_desc_valid_extend; auto.
+
+      safestep.
+      rewrite Data.avail_rep_split. cancel.
+      autorewrite with lists.
+      rewrite divup_1; rewrite <- entry_valid_ndata by auto.
+      apply helper_loglen_data_valid_extend; auto.
+
+      (* write header *)
+      safestep.
+      denote Hdr.rep as Hx; unfold Hdr.rep in Hx.
+      destruct_lift Hx.
+      unfold Hdr.hdr_goodSize in *; intuition.
+      eapply loglen_valid_goodSize_l; eauto.
+      eapply loglen_valid_goodSize_r; eauto.
+
+      (* sync content *)
+      step.
+      eauto 10.
+      prestep. norm. cancel. intuition simpl.
+      instantiate ( 1 := map ent_addr (padded_log new) ).
+      rewrite desc_padding_unsync_piff.
+      pred_apply; cancel.
+      rewrite map_length, padded_log_length; auto.
+      apply padded_desc_valid.
+      apply loglen_valid_desc_valid; auto.
+      eauto 10.
+
+      safestep.
+      autorewrite with lists.
+      rewrite entry_valid_ndata, Nat.mul_1_r; auto.
+      eauto 10.
+
+      (* sync header *)
+      safestep.
+      eauto 10.
+      step.
+
+      (* post condition *)
+      safestep.
+      or_l; cancel.
+      cancel_by extend_ok_helper; auto.
+      solve_checksums.
+
+      (* crash conditons *)
+      (* after sync data : Extended *)
+      cancel.
+      repeat xcrash_rewrite.
+      xform_norm. cancel. xform_normr. cancel.
+      or_r. cancel.
+      extend_crash.
+      solve_checksums.
+      solve_checksums.
+
+      cancel.
+      repeat xcrash_rewrite.
+      xform_norm; cancel. xform_normr; cancel.
+      or_r. cancel. extend_crash.
+      solve_checksums.
+      solve_checksums.
+
+      cancel.
+      repeat xcrash_rewrite.
+      xform_norm; cancel. xform_normr; cancel.
+      or_r. cancel. extend_crash.
+      solve_checksums.
+      solve_checksums.
+
+      cancel.
+      repeat xcrash_rewrite.
+      xform_norm; cancel. xform_normr; cancel.
+      or_r. cancel. extend_crash.
+      solve_checksums.
+      solve_checksums.
+
+      repeat xcrash_rewrite.
+      xform_norm; cancel. xform_normr; cancel.
+      or_r. cancel. extend_crash.
+      solve_checksums.
+      solve_checksums.
+
+      cancel.
+      repeat xcrash_rewrite.
+      xform_norm; cancel. xform_normr; cancel.
+      or_r. cancel. extend_crash.
+      solve_checksums.
+      solve_checksums.
+
+
+      (* before writes *)
+      cancel.
+      repeat xcrash_rewrite.
+      xform_norm; cancel. xform_normr; cancel.
+      or_l; cancel. extend_crash.
+      solve_checksums.
+
+      cancel.
+      repeat xcrash_rewrite.
+      xform_norm; cancel. xform_normr; cancel.
+      or_l; cancel.
+      rewrite Desc.avail_rep_merge. cancel.
+      rewrite map_length.
+      apply helper_loglen_desc_valid_extend; auto.
+      solve_checksums.
+
+      xcrash.
+      or_l; cancel.
+      solve_checksums.
+
+      xcrash.
+      or_l; cancel.
+      solve_checksums.
+
+    (* false case *)
+    - safestep.
+      or_r; cancel.
+      apply loglen_invalid_overflow; auto.
+      solve_checksums.
+
+    (* crash for the false case *)
+    - xcrash.
+      or_l; cancel.
+      solve_checksums.
+  Qed.
+
+
+  Hint Extern 1 ({{_}} Bind (avail _ _) _) => apply avail_ok : prog.
+  Hint Extern 1 ({{_}} Bind (read _ _) _) => apply read_ok : prog.
+  Hint Extern 1 ({{_}} Bind (trunc _ _) _) => apply trunc_ok : prog.
+  Hint Extern 1 ({{_}} Bind (extend _ _ _) _) => apply extend_ok : prog.
